\section{Introduction}

\begin{exercise}
	Recall that the number of $k$-subsets of $[n]$ is $\binom{n}{k}$. Given a $k$-subset $S = \{x_1,\ldots,x_k\}$ of $[n]$, we write $S_< = \{x_1,\ldots,x_k\}_<$ to denote that $x_1<x_2<\cdots<x_k$. Determine the number of $k$-subsets $\{x_1,\ldots,x_k\}_<$ of $[n]$ such that $x_i \cong i \mod 2$.
\end{exercise}
For example, for $n=6$ and $k=3$, we have the subsets $\{1,4,5\},\{1,2,3\},\{1,2,5\},\{3,4,5\}$.


Broadly, there are three types of ``answers'': a formula, a recurrence, and a generating function. A great example of the second and third is the following.\\
% Euler's Theorem
$p(n)$, the number of number partitions of $n$, is given by the generating function
\[ \sum_{n \ge 0} p(n) x^n = \prod_{i \ge 1} \frac{1}{1-x^i}. \]
Using this, a recursion may be obtained as well.
We do \emph{not} plug in values for $x$ in the above. We merely look at the coefficient of $x^n$ in it. We want the coefficient to be a finite sum for all $n$. If it is an infinite sum, convergence issues may arise.

% www.math.iitb.ac.in/~krishnan/phd-2022/

% The number of derangements of $[n]$ is the integer closest to $n!/e$.
% Bell number B_n (number of set partitions of $[n]$) : \sum_{n \ge 0} B_n x^n / n! = e^{e^x - 1}.

\subsection{Counting in \texorpdfstring{$\mathfrak{S}_n$}{Sn}}

	Recall that $\mathfrak{S}_n$ is generated by transpositions. A transposition $(i,j)$ is a permutation $\sigma$ defined by
	\[ \sigma(k) = \begin{cases} j, & k=i, \\ i, & k=j, \\ k, & \text{otherwise.} \end{cases} \]
	In fact, $\mathfrak{S}_n$ is generated by the set of just ``adjacent transpositions'' $S_i = (i,i+1)$ for $1 \le i < n$.
	We have
	\begin{align*}
		S_i^2 &= \Id \\
		S_i S_{i+1} S_i &= S_{i+1} S_i S_{i+1} \\
		S_i S_j &= S_j S_i \text{ if $|i-j| > 2$.}
	\end{align*}


	\begin{fdef}
		Given a permutation $\pi \in \mathfrak{S}_n$, define the \emph{length} $\ell(\pi)$ of $\pi$ to be the smallest $k$ such that there exist adjacent transpositions $\sigma_1,\cdots,\sigma_k$ such that $\pi = \sigma_1\cdots\sigma_k$.
	\end{fdef}
	% PRESENT PROOF THAT WE CAN WRITE IT IN THIS WAY ON TUESDAY -- 02/08/2022
	% DONE.

	\begin{fprop}
		Consider the \emph{inversion number} $\inv(\pi)$ of a permutation, defined by
		\[ \inv(\pi) = \left|\{ 1 \le i \le j \le n : \pi_i > \pi_j \}\right|. \]
		Then, $\ell(\pi) = \inv(\pi)$.
	\end{fprop}

	\begin{fdef}
		The \emph{sign} of a permutation $\pi$ is defined by $\sign(\pi) = (-1)^{\inv(\pi)}$. Equivalently,
		\[ \sign(\pi) = \frac{\prod_{1 \le i < j \le n} (x_{pi_i} - x_{\pi_j})}{\prod_{1 \le i < j \le n} (x_i - x_j)}. \]
	\end{fdef}

	% LATER, STUDY NUMBER OF ``REDUCED'' PRODUCTS? (NUMBER OF WAYS IN WHICH PI CAN BE WRITTEN AS A PRODUCT OF L(PI) ADJ TRANSPOSITIONS)


	It is straightforward to see that for all $\pi \in \mathfrak{S}_n$, $0 \le \inv(\pi) \le \binom{n}{2}$.
	\begin{fprop}
		\label{prop: inv n}
		Consider $\inv_n(q) = \sum_{\pi \in \mathfrak{S}_n} q^{\inv(\pi)}$. Then,
		\[ \inv_n(q) = \prod_{1 \le m \le n} [n]_q, \]
		where
		\[ [m]_q = \begin{cases} 1 + q + \cdots + q^{m-1}, & m \ge 1, \\ 0, & m = 0. \end{cases} \]
	\end{fprop}
	This quantity $[m]_q$ is called the $q$-analogue of $m$, and similarly, the $q$-analogue of $n!$ is $\prod_{i=1}^n [m]_q$ (this is slightly vague).
	Note in particular that $n! = \inv_n(1)$.
	\begin{proof}
		We prove this by induction. It is easily verified for $n = 2$.\\
		Take $\sigma \in \mathfrak{S}_{n-1}$. There are $n$ ``gaps'' where $n$ can be ``placed'' in $\sigma$ to get a permutation in $\mathfrak{S}_n$. If we place it in the $i$th position from the end (for $0 \le i \le n-1$), the inversion number of the newly obtained permutation is $i$ more than the inversion number of $\sigma$.\\
		As a result,
		\[ \inv_n(q) = \inv_{n-1}(q) + q \inv_{n-1}(q) + q^2 \inv_{n-1}(q) + \cdots + q^{n-1} \inv_{n-1}(q) = [n]_q \inv_{n-1}(q), \]
		where the $q^i \inv_{n-1}(q)$ term corresponds to the case where $n$ is placed in the $i$th position from the end. The required follows by the inductive hypothesis.
	\end{proof}

	\begin{definition}[Descent]
		For $\pi \in \mathfrak{S}_n$, define the \emph{descents} $\DES(\pi) = \{i \in [n-1] : \pi_i > \pi_{i+1}\}$, $\des(\pi) = |\DES(\pi)|$, and $\maj(\pi) = \sum_{i \in \DES(\pi)} i$. 
	\end{definition}
	There are central limit theorems for many of these parameters, which we shall not study.\\
	A permutation $\pi$ has $\des(\pi) + 1$ many ``increasing runs''.

	For example, for the permutation $\pi = (1\mapsto 5,2\mapsto1,3\mapsto2,4\mapsto6,5\mapsto4,6\mapsto3) \in \mathfrak{S}_6$, $\DES(\pi) = \{1,4,5\}$, $\des(\pi) = 3$, and $\maj(\pi) = 10$.

	\begin{fprop}
		\label{prop: maj n}
		The distribution of $\maj(\pi)$ over $\mathfrak{S}_n$ is the same as that of $\inv(\pi)$. Equivalently,
		\[ \maj_n(q) = \sum_{\pi \in \mathfrak{S}_n} q^{\maj(\pi)} = \prod_{m=1}^n [m]_q = \inv_n(q). \] 
	\end{fprop}
	This result took nearly 50 years to prove!
	\begin{proof}
		The strategy is similar to that of \Cref{prop: inv n}. Let $\pi \in \mathfrak{S}_{n-1}$. As before, there are $n$ positions to insert $n$.
		% An insertion increases $\maj$ (compared to $\pi$) only if it is placed in the middle of an increasing run. That is, we must place it  Further, in this case, it increases $\des$ by $1$. What is the sum of $\maj$ increases over all possible insertions? 
		\begin{itemize}
			\item Label the positions of descents of $\sigma$ and the last position from right ot left as $0,1,\ldots,\des(\pi)$.
			\item Label the remaining positions from left to right as $\des(\pi)+1,\ldots,n-1$.
		\end{itemize}
		We claim that inserting $n$ at a position increases $\maj$ by the labelled amount.\\
		If inserted anywhere, all the descent positions starting from there increase by $1$. This explains why the increase is equal to the labelled quantity for positions that are descents, since no new descents are introduced. In the case where we insert it in a position of non-descent, we further introduce a new descent at the position of insertion of $n$, which explains why the increase is equal tot he labelled quantity for positions that are not descents.\\
		The remainder of the proof is identical to that of \Cref{prop: inv n}, since the increases are in bijection with $[n-1]_0$.
	\end{proof}

	\begin{definition}
		A parameter $f : \mathfrak{S}_n \to \R$ of permutations such that
		\[ \sum_{\pi \in \mathfrak{S}_n} q^{f(\pi)} = \prod_{1 \le m \le n} [m]_q \]
		is said to be \emph{Mahonian}.
	\end{definition}

	As we saw in \Cref{prop: inv n,prop: maj n}, both $\inv$ and $\maj$ are Mahonian.

\subsection{Counting spanning trees}

	\begin{problem*}
		Count the number of spanning trees in an arbitrary (finite) graph $G$.
	\end{problem*}

	This was solved by Kirchhoff using the Matrix Tree Theorem.
	
	\begin{ftheo}[Matrix Tree Theorem]
		Consider the \emph{Laplacian} $L = D-A$ of a graph $G$, where $A$ is its adjacency matrix and $D$ is a diagonal matrix with the diagonal entries being the degrees of the vertices. The determinant of any $(n-1)\times(n-1)$ submatrix of $L$ obtained by omitting any arbirary row and column is equal to the number of spanning trees of $G$.
	\end{ftheo}

	% oriented incidence matrix is totally unimodular -- poincare

	In particular, when $G = K_n$, we end up getting the following.

	\begin{ftheo}[Cayley's Theorem]
		\label{theo: cayleys theorem}
		The number of spanningtrees in $K_n$ is $n^{n-2}$.
	\end{ftheo}
	One proof by Pr\"{u}fer gives an explicit bijection between spanning trees and sequences $(v_1,\ldots,v_{n-2})$ of vertices in $G$.\\
	Another proof is of course using the matrix tree theorem, which reduces it to a simple determinant calculation.\\
	Joyal gave another bijection between elements of the form $(T,u,v)$ where $T$ is a spanning tree and $u,v$ are vertices in $G$, and functions from $[n] \to [n]$.\\

	The proof we give uses exponential generating functions. Recall the following result, which we give without proof. Interested readers may consult Corollary 5.1.6 of \cite{ec2} for further details.

	\begin{ftheo}[Exponential Formula]
		\label{ec2: egf sum over partitions}
		Let $\{f_n\}$ be a sequence with exponential generating function
		\[ F(x) = \sum_{n \ge 1} f_n \frac{x^n}{n!}. \]
		Define the sequence $h_n$ by
		\[ h_n = \sum_{\substack{\pi \in \operatorname{SetPartn}([n]) \\ \pi = \{S_1,\ldots,S_k\}}} f_{|S_1|} f_{|S_2|} \cdots f_{|S_k|}  \]
		and $h_0 = 1$, and let
		\[ H(x) = \sum_{n \ge 0} h_n \frac{x^n}{n!}. \]
		Then,
		\[ H(x) = \exp(F(x)) \]
	\end{ftheo}
	Note that the summation of $F$ is for $n \ge 1$, because we may assume that $f_0 = 0$ since $f_0$ does not appear in the expression of any $h_n$.\\

	\begin{fdef}[Compositional inverse]
		Generating functions $F$ and $G$ are said to be \emph{compositional inverses} (of each other) if $F(G(x)) = G(F(x)) = x$.
	\end{fdef}

	Let
	\[ F(x) = \sum_{n \ge 0} f_n x^n \text{ and } G(x) = \sum_{n \ge 0} g_n x^n \]
	be compositional inverses of each other. It is reasonably straightforward to show that $f_0 = g_0 = 0$ and $f_1,g_1 \ne 0$. The first condition implies that the coefficient of any $x^n$ in $F\circ G$ (or $G \circ F$) is finite. 

	\begin{ftheo}[Lagrange Inversion Theorem]
		\label{theo: lagrange inversion}
		Let
		\[ F(x) = \sum_{n \ge 0} f_n x^n \text{ and } G(x) = \sum_{n \ge 0} g_n x^n \]
		be compositional inverses of each other. Then, $ng_n$ is the coefficient of $1/x$ in $(1/F(x))^n$.
	\end{ftheo}
	Equivalently, $ng_n$ is the coefficient of $x^{n-1}$ in $(x/F(x))^n$.
	\begin{proof}
		We have
		\[ x = G(F(x)) = \sum_{i \ge 0} g_i F(x)^i. \]
		Differentiating,
		\[ 1 = \sum_{i \ge 0} g_i i F(x)^{i-1} F'(x). \]
		As a result,
		\[ \left(\frac{1}{F(x)}\right)^n = \sum_{i \ge 0} g_i i F(x)^{i-1-n} F'(x).  \]
		Whenever $i \ne n$, the coefficient of $1/x$ in $F(x)^{i-1-n} F'(x) = \left(F(x)^{i-n}/(i-n)\right)'$ is zero. Indeed, recall that the coefficient of $1/x$ in the derivative of any power series with possibly negative exponents is zero.\\
		As a result, the coefficient of $1/x$ in $(1/F(x))^n$ is equal to the coefficient of $1/x$ in $g_n n F'(x) / F(x)$.
		% , which is the constant term in $n g_n x F'(x) / F(x)$ -- observe that there cannot be a $x^{-m}$ term for any $m \ge 2$.
		We have
		\[ \frac{F'(x)}{F(x)} = \frac{f_1 + 2f_2x + \cdots}{f_1x + f_2x^2 + \cdots}. \]
		The constant term in this is $f_1/f_1 = 1$, and the desideratum follows. 
	\end{proof}

	At long last, let us return to \nameref{theo: cayleys theorem}.

	\begin{proof}[Proof of \nameref{theo: cayleys theorem}]
		Instead of looking at the number $\text{T}_n$ of spanning trees, we shall look at $\text{RT}_n$, the number of \emph{rooted} spanning trees. Clearly, $\text{RT}_n = n \text{T}_n$.\\
		Define $\text{RF}_n$ to be the number of rooted forests on $[n]$ and let
		\begin{align*}
			\operatorname{RF}(x) &= \sum_{n \ge 0} \text{RF}_n \frac{x^n}{n!} \\
			\operatorname{RT}(x) &= \sum_{n \ge 0} \text{RT}_n \frac{x^n}{n!}.
		\end{align*}

		Using \Cref{ec2: egf sum over partitions}, it is not too difficult to see that
		\begin{equation}
			\label{eqn 1}
			\operatorname{RF}(x) = \exp(\operatorname{RT}(x)).
		\end{equation}

		\textbf{Claim} (Polya). $\text{RT}_{n+1} = (n+1) \text{RF}_n$.\\
		Indeed, any rooted tree on $K_{n+1}$ may be obtained from a rooted forest $F$ on $K_n$ by adding a new vertex $v$, adding the edge between each root in $F$ and $v$ to the spanning tree, removing the ``root status'' from all vertices except $v$. $v$ can be labelled in $n+1$ ways, so we are done.\\

		As a result,
		\begin{equation}
			\label{eqn 2}
			\operatorname{RF}(x) = \sum_{n\ge 0} \frac{\operatorname{RT}_{n+1}}{n+1} \cdot \frac{x^n}{n!} = \frac{1}{x} \operatorname{RT}(x).
		\end{equation}
		Combining \Cref{eqn 1,eqn 2},
		\[ \operatorname{RT}(x) = x \exp(\operatorname{RT}(x)). \]
		That is, $\operatorname{RT}$ is the compositional inverse of $x \mapsto xe^{-x}$.
		Now, we use the \nameref{theo: lagrange inversion} to get that $n\text{RT}_n/n!$ is equal to the coefficient of $x^{n-1}$ in $(x/xe^{-x})^n = e^{nx}$, which is $n^{n-1}/(n-1)!$. Therefore, $\text{T}_n = \text{RT}_n/n = n^{n-2}$ and we are done.
	\end{proof}

	% cool fact: matching polynomial of any graph has real roots.

\subsection{Chebyshev polynomials}

	We would like a polynomial $T_n(x)$ such that $T_n(\cos\theta) = \cos(n\theta)$. Why does such a polynomial even exist? Recall that
	\[ (\cos \theta + \iota \sin \theta)^n = \cos n\theta + \iota \sin n\theta. \]
	Since the real part of the left only has even powers of $\sin$, we can convert it to a polynomial of $\cos\theta$s alone.\\
	For example,
	\begin{align*}
		T_0(x) &= 1, \\
		T_1(x) &= x, \\
		T_2(x) &= 2x^2-1.
	\end{align*}

	\begin{fprop}
		\[ T_n(x) = \begin{cases} 1, & n=0, \\ x, & n=1, \\ 2xT_{n-1}(x) - T_{n-2}(x), & n \ge 2. \end{cases} \]
	\end{fprop}
	We give the proof of the above in the solution to \Cref{problem: recurrence of Chebyshev of the first kind}.

	% % PSHEET 2 EXERCISE 1
	% \begin{ftheo}
	% 	Show that
	% 	\[ T_n(x) = 2xT_{n-1}(x) - T_{n-2}(x). \]
	% 	when $n \ge 2$, and $T_0(x) = 1, T_1(x) = x$.
	% \end{ftheo}

	\begin{fdef}[Chebyshev polynomials]
		The $n$th \emph{Chebyshev polynomial of the first kind} $T_n$ is defined as above.\\
		The $n$th \emph{Chebyshev polynomial of the second kind} $U_n$ is defined by
		\[ U_n(x) = \begin{cases} 1, & n=0, \\ 2x, & n=1, \\ 2xU_{n-1}(x) - U_{n-2}(x), & n \ge 2. \end{cases} \]
	\end{fdef}


	% \begin{exercise}
	% 	Show that
	% 	\begin{enumerate}
	% 		\item \phantom{pain}
	% 		\begin{enumerate}[label=\alph*)]
	% 			\item $T_n(1) = 1$.
	% 			\item $T_n(-1) = (-1)^n$
	% 		\end{enumerate}
	% 		\item \phantom{pain}
	% 		\begin{enumerate}[label=\alph*)]
	% 			\item $U_n(1) = n+1$.
	% 			\item $U_n(-1) = (-1)^n(n+1)$
	% 		\end{enumerate}
	% 		\item $U_n(\iota/2)/\iota^{n}$ is the $(n+1)$th Fibonacci number.
	% 		\item if $m,n \ge 1$,
	% 		\[ T_{m+n}(x) = T_m(x)U_n(x) - T_{m-1}(x)U_{n-1}(x) \]
	% 	\end{enumerate}
	% \end{exercise}

	Consider the number of tilings of a $1\times n$ board $B_n$ using squares ($1\times 1$ pieces) and dimers ($1\times 2$ pieces). It is not too difficult to show that this corresponds to the Fibonacci numbers.\\
	Now, instead consider a \emph{weighted} version of this problem, where we give squares a weight of $2x$ and dimers a weight of $-1$. The weight $\wt(T)$ of a given tiling $T$ is equal to the product of the weights of the pieces used. Then, the Chebyshev polynomial $U_n$ is just the sum of the weights of all tilings of $B_n$!
	\[ U_n(x) = \sum_{\text{tilings $T$ of $B_n$}} \wt(T). \]


	Given a tiling $T$, let $S(T)$ and $D(T)$ be the number of squares and dimers in the tiling respectively.
	In general, define
	\[ F_n(s,t) = \sum_{\text{tilings $T$ of $B_n$}} s^{S(T)} t^{D(T)}. \]

	Then,
	\begin{align*}
		F_0(s,t) &= 1, \\
		F_1(s,t) &= s, \\
		F_n(s,t) &= sF_{n-1}(s,t) + tF_{n-2}(s,t).
	\end{align*}

\subsection{More on $q$-analogues}

	Recall the definition of $[n]_q! = \prod_{i=1}^n [i]_q$. Inspired by this, define
	\[ \binom{n}{k}_q = \frac{[n]_q!}{[k]_q[n-k]_q!}. \]
	This is clearly a rational function of $q$. It turns out that this is a polynomial in $q$! For example,
	\[ \binom{5}{2}_q = \frac{[5]_q[4]_q}{[2]_q[1]_q} = 1 + q + 2q^2 + 2q^3 + 2q^4 + q^5 + q^6. \]

	Recall that
	\[ \binom{n}{k} = \binom{n-1}{k-1} + \binom{n-1}{k}. \]

	\begin{exercise}
		Show that
		\[ \binom{n}{q}_q = q^k \binom{n-1}{k}_q + \binom{n-1}{k-1}_q = \binom{n-1}{k}_q + q^{n-k} \binom{n-1}{k-1}_q . \]
	\end{exercise}
	These are called the $q$-Pascal's recurrences.

	\begin{fcor}
		$\binom{n}{k}_q$ is a polynomial. in $q$ with non-negative coefficients.
	\end{fcor}
	It turns out that the coefficients of the polynomial are unimodal and symmetric! We do not prove this, the reader can see \_ for more details.
	% zeinberger, AMM (katyohara?)

	% sperner's theorem(?) : maximal UNIQUE antichain is the binom(n)(n/2) in the middle of the poset

	A natural question to ask then is: what do the coefficients of this polynomial count?\\
	Let $\binom{n}{k}_q = f_{n,k}(q) = \sum_{r \ge 0} a_{n,k}^{(r)} q^r$.
	Can we have
	\[ \binom{n}{k}_q = \sum_{T \in \binom{[n]}{k}} q^{\operatorname{parameter}(T)}? \]
	$a_{n,k}^{(r)}$ then just counts the number of $T$ with the given parameter value.\\
	Recall that $\binom{n}{k}$ is the number of paths from $(0,0)$ to $(n-k,k)$ if only upwards and rightwards movements on the integer lattice $\Z^2$ are allowed. Let $P$ be such a path.\\
	% \prod q^{(x_{i+1}-x_i-1)}
	% number partitions -- ``ferrer's diagram''
	Consider the portion of the box above $P$. This can be viewed as the Ferrer diagram of some number partition $\lambda(P)$. $\lambda(P)$ has at most $k$ parts, and no part is of size more than $n-k$. In fact, \emph{all} such partitions correspond to some path!\\
	What number is $\lambda(P)$ a number partition of? Denote this number as $|\lambda(P)|$. Let $S_{n,k}$ be the set of all paths of the mentioned form. 

	\begin{ftheo}
		\[ \sum_{P \in S_{n,k}} q^{|\lambda(P)|} = \binom{n}{k}_q. \]
	\end{ftheo}
	Surprisingly, the proof of the above is near-straightforward using the $q$-Pascal recurrence -- merely consider two cases depending on whether the first step of the path is right or upwards.

\subsection{Derivative polynomials}

	We begin this section by recalling the following rather interesting result.\\
	Define the \emph{Bell polynomial} $B_{n,k}$ by
	\[ B_{n,k}(x_1,x_2,\ldots,x_{n-k+1}) = \sum \frac{n!}{j_1! (1!)^{j_1} j_2! (2!)^{j_2} \cdots j_{n-k+1}! ((n-k+1)!)^{n-k+1}} \cdot x_1^{j_1} x_2^{j_2} \cdots x_{n-k+1}^{j_{n-k+1}}, \]
	where the summation is taken over all indices $j_1,\ldots,j_{n-k+1}$ of non-negative integers such that
	\begin{align*}
		k &= j_1 + j_2 + \cdots + j_{n-k+1} \text{ and} \\
		n &= j_1 + 2j_2 + 3j_3 + \cdots + (n-k+1)j_{n-k+1}.
	\end{align*}
	This has a natural correspondence to the Stirling numbers of the second kind, with $j_i$ representing the number of partitions of size $i$. In particular, the sum of coefficients of $B_{n,k}$ is $S_{n,k}$.

	\begin{fprop}[Fa\`{a} di Bruno's Formula,\cite{faadibruno}]
		\[ D^n f(g(x)) = \sum f^{(k)}(g(x)) \cdot B_{n,k} (g'(x), g''(x), \ldots, g^{(n-k+1)}(x)). \]
	\end{fprop}

	To illustrate this better, let us look at the first few derivatives explicitly. Dropping the $(x)$ on the right to make the notation more succinct, we have
	\begin{align*}
		Df(g(x)) &= f'(g) g' \\
		D^2f(g(x)) &= f''(g) (g')^2 + f'(g) g'' \\
		D^3f(g(x)) &= f'''(g) (g')^3 + 3 f''(g) g' g'' + f''(g) g'''.
	\end{align*}
	Consider the partitions of $\{1,2,3\}$, given by $1|2|3$, $12|3$, $13|2$, $23|1$, and $123$. The number of partitions of $[n]$ with $n_i$ parts of size $i$ for each $i$ neatly corresponds to the coefficient of $\prod_i (g^{(i)})^{n_i}$!

	% Faa di Bruno's formula
	% Df(g(x)) = f'(g) g'
	% D^2 = f''(g)(g')^2 + f'(g)g''
	% D^3 = f'''(g) (g')^3 + 3 f''(g)(g')(g'') + f''(g)g''' -- 1|2|3 ; 12|3 13|2 12|3 ; 123
	% coefficients relate to Bell numbers!
	% even a multivariate version that relates to multivariate partitions (?)

	Let $y = f(x)$. If $Dy = p(f(x))$ for some polynomial $p$, then $D^ny$ is a polynomial of $f$ as well.\\
	Suppose that $D^ny = p_n(y)$ for some sequence of polynomials $(p_n)$.
	\begin{exercise}
		Show that
		\begin{align*}
			p_0(y) &= y \\
			p_n(y) &= \begin{cases} y & n=0 \\ p_{n-1}(y) \cdot p_1(y) & n \ge 1. \end{cases}
		\end{align*}
	\end{exercise}

	For the remainder of this section, set $y = \tan x$ and $z = \sec x$. Then, $Dy = 1+y^2 = z^2$ and $Dz = yz$. It is not difficult to see that
	\begin{align*}
		D^2y &= 2yz^2 \\
		D^3y &= 4y^2z^2 + 2z^4 \\
		D^4y &= 8y^3z^2 + 16yz^4
	\end{align*}

	\begin{exercise}
		With $y,z$ defined as above, show that
		\begin{enumerate}
			\item $D^ny$ is a homogeneous polynomial in $y,z$ of degree $(n+1)$.
			\item $D^ny$ has only terms with even exponents of $z$.
		\end{enumerate}
	\end{exercise}

	\begin{fcor}
		We can write $D^ny = \sum_{k=0}^{\lfloor (n-1)/2 \rfloor} W_{n,k} z^{2k+2} y^{n-2k-1}$.
	\end{fcor}

	\begin{exercise}
		Prove or disprove that
		\[ \sum W_{n,k} = n!. \]
	\end{exercise}
	Again, we ask the question: is there some parameter on $\pi \in \mathfrak{S}_n$ such that
	\[ W_n(x) = \sum_{k = 0}^{\lfloor (n-1)/2 \rfloor} W_{n,k} x^k = \sum_{\pi \in \mathfrak{S}_n} x^{\operatorname{parameter}(\pi)}? \]

	\begin{fdef}[Peak]
		Given a permutation $\pi \in \mathfrak{S}_n$, we say that $i \in [n] \setminus \{1,n\}$ is a \emph{peak} of $\pi$ if $\pi_i > \pi_{i-1}$ and $\pi_i > \pi_{i+1}$. Denote the set of peaks of $\pi$ by $\Peak(\pi)$, $\pk(\pi) = |\Peak(\pi)|$ the number of peaks.
	\end{fdef}

	\begin{lemma}
		\label{lem: Wnk recurrence}
		Show that
		\[ W_{n,k} = (2k+2) W_{n-1,k} + (n-2k) W_{n-1,k-1}. \]
		for $n,k \ge 1$.
	\end{lemma}
	\begin{proof}
		We have
		\begin{align*}
			D^{n}y &= D \sum_{k=0}^{\lfloor (n-2)/2 \rfloor} W_{n-1,k} z^{2k+2} y^{n-2k-2} \\
				&= \sum_{k=0}^{\lfloor (n-2)/2 \rfloor} (2k+2) W_{n-1,k} z^{2k+1} \cdot zy \cdot y^{n-2k-2} + (n-2k-2) W_{n-1,k} z^{2k+2} y^{n-2k-3} \cdot z^2 \\
				&= \sum_{k=0}^{\lfloor (n-2)/2 \rfloor} (2k+2) W_{n-1,k} z^{2k+2} y^{n-2k-1} + (n-2k-2) z^{2k+4} y^{n-2k-3}.
		\end{align*}
		The required follows.
	\end{proof}

	\begin{ftheo}
		\[ W_n(x) = \sum_{\pi \in \mathfrak{S}_n} x^{\pk(\pi)}. \]
	\end{ftheo}
	\begin{proof}
		Let $Y_n$ be the polynomial on the right, and let $Y_{n,k}$ be its coefficients. It is easily checked that $Y_{n,k}$ and $W_{n,k}$ are equal for $n=0$ or $k=0$. To prove the statement, we shall merely show that $Y_{n,k}$ satisfies the recurrence of \Cref{lem: Wnk recurrence} too.\\
		Similar to what we did in earlier proofs such as those of \Cref{prop: inv n,prop: maj n}, let $\sigma$ be a permutation in $\mathfrak{S}_{n-1}$.\\ We shall use it to get a permutation $\pi \in \mathfrak{S}_n$ by ``inserting'' $n$ at one of the $n$ possible positions. If we insert it at the position of a non-peak of $\sigma$, the number of peaks increases by one. If we insert it before or after the position of a peak, the number of peaks stays the same. Since peaks cannot occur immediately after each other, we can insert it at precisely $2k+2$ positions while ensuring that the number of peaks does not increase (the extra $2$ is for the extreme positions), and so at $n-2k-2$ positions which increases the number of peaks by one. Therefore,
		\[ Y_{n,k} = (2k+2)Y_{n-1,k} + (n-2(k-1)-2)Y_{n-1,k-1} = (2k+2) Y_{n-1,k} + (n-2k)Y_{n-1,k-1}. \]
	\end{proof}
	\begin{problem}
		\begin{enumerate}
			\item Show that
			\[ W_{n,k} = \_ W_{n-1,k} + \_ W_{n-1,k-1}. \]
		\end{enumerate}
	\end{problem}

	% z = sec x, Dz = yz.

\subsection{Matching Theory}

	\begin{fdef}[Matching]
		Given a graph $G = (V,E)$, a \emph{matching} in $G$ is a collection $M \subseteq E$ of edges such that for any distinct $e_1,e_2 \in M$, $e_1 \cap e_2 = \emptyset$.\\
		Denote the number of $k$-sized matchings by $m_k(G)$. Define the \emph{matching polynomial}
		\[ \Match_G(x) = \sum_{k \ge 0} m_k(G) x^k \]
	\end{fdef}

	Some authors also define the polynomial as
	\[ N_G(x) = \sum_{k \ge 0} (-1)^k m_k(G) x^{n-2k}. \]
	Clearly, $N_G(x) = x^n \cdot \Match_G(-1/x^2)$.\\

	There is a very rich literature regarding matching theory. One work that set off a frenzy of results in related areas was \cite{Edmonds1965MaximumMA}, which gave a polynomial-time algorithm to get a maximum weight matching in any graph. It does so by looking at the polytope in $\R^{E}$ that is the convex hull of the indicator functions of all matchings.
	It is worth noting that while there is a polynomial time algorithm to find a maximum weight matching, the problem of determining the number of maximum matchings in a graph is \textsf{\#P}-complete.

	% convex hull of (01) vectors of matchings in R^{|E|} due to edmonds. this is linear program, so we can get a non-linear programming way. this gives a method to get a maximum weight matching!!! (place any weights you want on edges)
	% counting number of matchings is #P-complete though.